## 4.35
Note in the below proof I work entirely in the domain of pure states. I am unsure if this failure to consider mixed states implies the proof is incomplete nor am I sure how the modified proof would look. Further thinking is necessary.

Since the vectors $`\ket{ij}`$ for $`i,j \in\{0,1\}`$ span the two qubit pure state space, an arbitrary two qubit pure state may be written $`\ket{\psi}=a\ket{0}\ket{v} + b\ket{1}\ket{w}`$ where $`|a|^2+|b|^2=1`$*. 
Therefore, the action of the classically controlled circuit (RHS) on $\ket{\psi}$ is to produce the state $`\ket{0}\ket{v}`$ with probability $`|a|^2`$ and the state $`\ket{1}U\ket{w}`$ with probability $`|b|^2`$. Our job is to verify that the quantum controlled circuit behaves identically. 

Prior to measurement in the LHS circuit, the state of the system is given by $`\ket{\psi}'=a\ket{0}\ket{v} + b\ket{1}U\ket{w}`$. We then measure with operators $`\ket{0}\bra{0}\otimes I`$ and $`\ket{1}\bra{1}\otimes I`$ with probabilities $`p(1)`$ and $`p(-1)`$ respectively.  
```math
p(1)= (a^*\bra{0}\bra{v} + b^*\bra{1}\bra{w}U^\dagger)\ket{0}\bra{0}\otimes I (a\ket{0}\ket{v} + b\ket{1}U\ket{w})=|a|^2
```
and the PM state is 
```math
\frac{1}{|a|}\ket{0}\bra{0}\otimes I (a\ket{0}\ket{v} + b\ket{1}U\ket{w})=\frac{a}{|a|}\ket{0}\ket{v} \sim \ket{0}\ket{v}
```
Similarly we find that $`p(-1)=|b|^2`$ and the associated PM state is $`\ket{1}U\ket{w}`$. We conclude that the quantum controlled circuit behaves identically to the classical control.

\* Let $`\ket{\psi}=\sum_{ij\in\{0,1\}}x_{ij}\ket{i}\ket{j}`$ where $`\sum_{ij\in\{0,1\}} |x_{ij}|^2=1`$. We can rewrite this as:
```math
\begin{align*}
&\sum_{ij\in\{0,1\}}x_{ij}\ket{i}\ket{j}=\ket{0}\sum_{j\in\{0,1\}}x_{0j}\ket{j}+\ket{1}\sum_{j\in\{0,1\}}x_{1j}\ket{j}\\
&=\frac{\sqrt{\sum_j|x_{0j}|^2}}{\sqrt{\sum_j|x_{0j}|^2}}\ket{0}\sum_{j\in\{0,1\}}x_{0j}\ket{j} + \frac{\sqrt{\sum_j|x_{1j}|^2}}{\sqrt{\sum_j|x_{1j}|^2}}\ket{1}\sum_{j\in\{0,1\}}x_{1j}\ket{j}
\end{align*}
```
then set
```math
\begin{align*}
a=\sqrt{\sum_j|x_{0j}|^2} \tag{1}
\end{align*}
```
```math
\begin{align*}
b = \sqrt{\sum_j|x_{1j}|^2} \tag{2}
\end{align*}
```
```math
\begin{align*}
\ket{v}= \sum_{j\in\{0,1\}}\frac{x_{0j}}{\sqrt{\sum_j|x_{0j}|^2}}\ket{j} \tag{3}
\end{align*}
```
```math
\begin{align*}
\ket{w}= \sum_{j\in\{0,1\}}\frac{x_{1j}}{\sqrt{\sum_j|x_{1j}|^2}}\ket{j} \tag{4}
\end{align*}
```
to get $`|a|^2+|b|^2=1`$ and $`\braket{v|v}=\braket{w|w}=1`$, completing the proof.