## 4.8
(1)\
I discarded my original proof in favour of the one that proceeds because it was comparatively more complicated, however, I drew a lot of good insights while working on it and you may find it instructive to [read](cheekycheats/4.8(1)_original_proof.md).

Our first order of business is to show that any 2x2 Hermitian matrix can be written, $K=\alpha I +\hat{r}\cdot\vec{\sigma}$ where $\alpha\in \mathbb{R}$ and $\hat{r} = (r_1,r_2,r_3)^T \in \mathbb{R}^3$. Suppose
$`K = 
\begin{pmatrix}
a & b\\
c & d
\end{pmatrix}`$,

$$
K= K^\dagger\rightarrow
\begin{pmatrix}
a & b\\
c & d
\end{pmatrix} =
\begin{pmatrix}
a^* & c^* \\
b^* & d^*
\end{pmatrix}\\
\rightarrow a,d \in \mathbb{R} \text{ and } b = c^*
$$

Define $\alpha$ and $r_3$ such that $a=\alpha +r_3$ and $d=\alpha-r_3$, and define $r_1$ and $r_2$ such that $b=r_1-ir_2$, then 

$$
K = 
\begin{pmatrix}
\alpha+r_3 & r_1-ir_2\\
r_1+ir_2 & \alpha-r_3
\end{pmatrix}\\
= \alpha I + 
\begin{pmatrix}
r_3 & r_1-ir_2\\
r_1+ir_2 & -r_3
\end{pmatrix}\\
=\alpha I +\hat{r}\cdot\vec{\sigma}
$$

In exercise 2.56, we showed that any unitary $U$ can be written $U = \exp(iK)$ where $K$ is Hermitian so, it follows from our previous work that any single qubit unitary can be written $U=\exp(i(\alpha I +\hat{r}\cdot\vec{\sigma}))$. By the spectral theorem we can decompose $\hat{r}\cdot\vec{\sigma}$ into its eigenvalues and eigenvectors as follows: $\hat{r}\cdot\vec{\sigma}=v\ket{v}\bra{v}+w\ket{w}\bra{w}$ and therefore

$$
\begin{align*}
&\exp(i(\alpha I +\hat{r}\cdot\vec{\sigma}))=\exp(i(v+\alpha)\ket{v}\bra{v}+i(w+\alpha)\ket{w}\bra{w})\\
&=e^{i(v+\alpha)}\ket{v}\bra{v}+e^{i(w+\alpha)}\ket{w}\bra{w}\\
&=e^{i\alpha}(e^{iv}\ket{v}\bra{v}+e^{iw}\ket{w}\bra{w})\\
&=e^{i\alpha}\exp(i\hat{r}\cdot\vec{\sigma})
\end{align*}
$$

Now define $\hat{n}=\hat{r}/||\hat{r}||$ and $\theta = -2||\hat{r}||$ to get 

$$
U = e^{i\alpha}\exp(-i\theta\hat{n}\cdot \vec{\sigma}/2)=e^{i\alpha}R_{\hat{n}}(\theta)
$$

(2)\
Let $\alpha=\pi/2, \theta=\pi$ and $\hat{n}=(1/\sqrt{2}, 0, 1/\sqrt{2})^T$ where $\hat{n}^T\cdot\hat{n}=1$.

$$
\begin{align*}
&e^{i\alpha}R_{\hat{n}}(\theta)=e^{i\pi/2}(\cos(\pi/2)I - i/\sqrt{2}\sin(\pi/2)(X+Z))\\
&=i\left(\frac{-i}{\sqrt{2}}(X+Z)\right) = 1/\sqrt{2}(X+Z)\\
&=H
\end{align*}
$$

(3)\
Let $\alpha=\pi/4, \theta=\pi/2$ and $\hat{n}=(0,0,1)$.

$$
\begin{align*}
&e^{i\alpha}R_{\hat{n}}(\theta)=e^{i\pi/4}(\cos(\pi/4)I-i\sin(\pi/4)Z)\\
&=e^{i\pi/4}
\begin{pmatrix}
\cos(\pi/4)-i\sin(\pi/4) & 0\\
0 & \cos(\pi/4)+i\sin(\pi/4)
\end{pmatrix}\\
&= e^{i\pi/4}
\begin{pmatrix}
e^{-i\pi/4} & 0\\
0 & e^{i\pi/4}
\end{pmatrix} =
\begin{pmatrix}
1 & 0\\
0 & i
\end{pmatrix}\\
&=S
\end{align*}
$$

