## 4.20

The LHS circuit can be described $`H_1H_2CNOT_{12}H_2H_1`$.
```math
\begin{align*}
H_1H_2CNOT_{12}H_2H_1&=H_1(\ket{0}\bra{0}\otimes I + \ket{1}\bra{1}\otimes Z)H_1\\
&=H_1(I\otimes\ket{0}\bra{0} + Z\otimes\ket{1}\bra{1})H_1\\
&=I\otimes\ket{0}\bra{0} + X\otimes\ket{1}\bra{1}\\
&=CNOT_{21}
\end{align*}
```
where we proved equality 2 in exercise 4.18. With this in mind, let's consider the effect of $`CNOT`$ on the $`\ket{\pm}`$ basis.

4.24
```math
\begin{align*}
CNOT_{12}\ket{+}\ket{+}&=CNOT_{12}H_1H_2\ket{0}\ket{0}\\
&=H_1H_2CNOT_{21}\ket{0}\ket{0}\\
&=\ket{+}\ket{+}
\end{align*}
```
where the second equality follows from the cricuit equality we just showed.

4.25
```math
CNOT_{12}\ket{-}\ket{+}=H_1H_2CNOT_{21}\ket{1}\ket{0} =\ket{-}\ket{+}
```

4.26
```math
CNOT_{12}\ket{+}\ket{-}=H_1H_2CNOT_{21}\ket{0}\ket{1} =\ket{-}\ket{-}
```

4.27
```math
CNOT_{12}\ket{-}\ket{-}=H_1H_2CNOT_{21}\ket{1}\ket{1} =\ket{+}\ket{-}
```